src/bubble-sort.dfy
@@ -1,14 +1,4 @@
-predicate sorted_between(A:array<int>, from:int, to:int)
-    reads A
-{
-    forall i, j :: from <= i < j < to && 0 <= i < j < A.Length ==> A[i]<=A[j]
-}
-
-predicate sorted(A:array<int>)
-    reads A
-{
-    sorted_between(A, 0, A.Length-1)
-}
+include "../src/sorted.dfy"
 
 method BubbleSort(A:array<int>)
     modifies A
