README.md
@@ -1,2 +1,16 @@
 # dafny-algorithms
 Common algorithms done in Dafny.
+
+## Coding
+IDE: Visual Studio Code.
+Extensions: Dafny.
+    Link: https://marketplace.visualstudio.com/items?itemName=correctnessLab.dafny-vscode
+
+## Run
+Right click on the .dfy file you want to run, then click on Dafny: Compile and Run.
+
+## Algorithms
+BinarySearch
+BubbleSort
+InsertionSort
+Nats
